Let $n$ denote the total number of tests she took. Let $s$ denote the sum of all her scores. Danielle's mean score when all scores are included is:
\begin{align*}
\frac{s}{n} = 85
\end{align*}
Danielle's mean score when the lowest grade is excluded is:
\begin{align*}
\frac{s-61}{n-1} = 88
\end{align*}
This yields a linear system of two equations in two unknowns $s$ and $n$:
\begin{align*}
s - 85n & = 0 \\
s - 88n  + 27 & = 0
\end{align*}
Since we want to solve for $n$, we'll substitute $s$ from the first equation into the second:
\begin{align*}
85n - 88n  + 27 = 0 \Rightarrow 3n = 27 \Rightarrow n = 9
\end{align*}
\begin{empheq}[box={\mathbox[colback=white]}]{equation*}
    9 ~\text{tests}
\end{empheq}