\documentclass[12pt]{article}
\newif\ifanswer\answertrue%\answerfalse% comment out to show/hide answers
\usepackage{../preamble3}% preamble always after \newif\ifanswer
\renewcommand{\theenumi}{\alph{enumi}}
%\pagenumbering{gobble}
\title{Flintridge Prep Summer School, Algebra II \\ June-July 2021}
\author{Patrick \& James Toche}
\date{Revised:~\today}

\begin{document}
\subsubsection*{Linear Equations}
\begin{align*}
  ax + bx & = c \\
        y & = \alpha + \beta x \\
y - y_{0} & = \beta (x - x_{0})
\end{align*} 

\subsubsection*{Quadratic Equations}
\begin{align*}
y & = a x^2 + b x + c \\
y & = a (x-h)^2 + k \\
y & = a (x-r_{1}) (x-r_{2}) \\[1ex]
r_{1}, r_{2}
  & = \frac{-b \pm \sqrt{b^2 - 4ac}}{2a} \\
h & = - \frac{b}{2a}, \quad k = - \frac{b^2-4ac}{4a^2}
\end{align*} 

\subsubsection*{Completing the Square}
\begin{align*}
y & = a x^2 + b x + c \\
  & = a \left(x^2 + \frac{b}{a} x +  \frac{c}{a}\right) \\[1ex]
  & = a \left[\left(x + \frac{b}{2a}\right)^2 - \left(\frac{b}{2a}\right)^2  + \frac{c}{a}\right] \\[1ex] 
  & = a \left[\left(x + \frac{b}{2a}\right)^2 - \frac{b^2-4ac}{(2a)^2}\right] \\[1ex] 
  & = a \left(x-\frac{-b - \sqrt{b^2 - 4ac}}{2a}\right) \left(x-\frac{-b + \sqrt{b^2 - 4ac}}{2a}\right)
\end{align*}

\subsubsection*{Ellipses}
\begin{align*}
& \text{major axis:} \;\qquad 2a = V_{1}V_{2} \\
& \text{minor axis:} \;\qquad 2b = coV_{1}coV_{2}\\
& \text{focal distance:} \quad 2c = F_{1}F_{2}\\
& a^2 = b^2 + c^2 \\
& \text{x-major:}\qquad \frac{(x-h)^2}{a^2} + \frac{(y-k)^2}{b^2} = 1 \\
& \text{y-major:}\qquad \frac{(x-h)^2}{b^2} + \frac{(y-k)^2}{a^2} = 1 
\end{align*}

\subsubsection*{Hyperbolas}
\begin{align*}
\text{x-major:}\quad \frac{(x-h)^2}{a^2} - \frac{(y-k)^2}{b^2} = 1 
\qquad\text{asymptotes:}\quad y = \pm \frac{b}{a}x \\
\text{y-major:}\quad \frac{(y-k)^2}{a^2} - \frac{(x-h)^2}{b^2} = 1 
\qquad\text{asymptotes:}\quad y = \pm \frac{a}{b}x \\
\end{align*}

\subsubsection*{Circles}
\begin{align*}
(x-h)^2 + (y-k)^2 = r^2
\end{align*}


\subsubsection*{Arithmetic Series}
\begin{align*}
a_{k} & = a_{1} + (k-1)d \\
      & = a_{n} - (n-k)d \\[1ex]
s_{n} & = na_{1} +\frac{n(n-1)d}{2} \\
      & = na_{n} -\frac{n(n-1)d}{2} \\
      & = \frac{n(a_{1}+a_{n})}{2} \\[1ex]
1 + 2 + 3 + \ldots + n & = \frac{n(n+1)}{2}
\end{align*}

\subsubsection*{Geometric Series}
\begin{align*}
a_{n} & = a_{1} r^{n-1} \\[1ex]
s_{n} & = a_{1} \frac{1-r^{n+1}}{1-r} 
\qquad\longrightarrow\qquad
s_{\infty} = \frac{a_{1}}{1-r} 
\end{align*}

\subsubsection*{Binomial Expansion}
\begin{align*}
(a+b)^{n} 
  & = 
  \binom{n}{0} a^{n}b^{0} 
+ \binom{n}{1} a^{n-1}b^{1} 
+ \binom{n}{2} a^{n-2}b^{2} 
+ \ldots 
%+ \binom{n}{n-2} a^{2}b^{n-2} 
+ \binom{n}{n-1} a^{1}b^{n-1} 
+ \binom{n}{n} a^{0}b^{n} \\[1ex]
\binom{n}{k} 
  & = \frac{n!}{k!(n-k)!} \\
\end{align*}

\subsubsection*{Law of Cosines}
\begin{align*}
a^2 = b^2 + c^2 - 2bc\, \cos(\alpha)
\end{align*}

\subsubsection*{Law of Sines}
\begin{align*}
\frac{\sin(\alpha)}{a} = \frac{\sin(\beta)}{b} 
\end{align*}

\subsubsection*{Triangles}
Area of a triangle with side lengths $a$, $b$, $c$:
\begin{align*}
\frac{1}{4} \sqrt{(2ab)^2 - \left(a^2+b^2-c^2\right)^2}
\end{align*}

\end{document}
