Let $F$ denote the midpoint of $BC$. 

\begin{figure}[H]
\centering
\includegraphics[width=0.6\linewidth]%
{pset-7-06-figure-01}
\caption{\label{pset:7:06:fig:1}}
\end{figure}


Distance $EF$ is the height of the right triangle $\triangle BFE$. 
\begin{align*}
EF^{2} + 6^{2} = 10^{2}
\end{align*}

Distance $EF$ is also the height of the right triangle $\triangle AFE$. 
\begin{align*}
EF^{2} + (AB+6)^{2} = AE^{2}
\end{align*}

Combining the two equation to eliminate $EF^{2}$ gives:
\begin{align*}
10^{2} - 6^{2} + (AB+6)^{2} = AE^{2}
\implies 
AB^{2} + 12AB + 10^{2} = AE^{2}
\end{align*}


The perimeter of triangle $\triangle BEC$ is:
\begin{align*}
BE + EC + BC
= 10 + 10 + 12
= 32
\end{align*}

The perimeter of triangle $\triangle AED$ is:
\begin{align*}
AE + ED + AD
= 2 AE + 2 (AB+6)
\end{align*}

Since perimeter of triangle $\triangle AED$ is twice the perimeter of triangle $\triangle BEC$:
\begin{align*}
AE + (AB+6) = 32
\implies
AE + AB = 26
\implies
AE^{2} 
= (26-AB)^{2}
= 26^{2} - 52AB + AB^{2}
\end{align*}

Substituting back:
\begin{align*}
AB^{2} + 12AB + 10^{2} 
  = AE^{2} 
& = 26^{2} - 52AB + AB^{2}
\\
\implies 
64AB 
& = 26^{2} - 10^{2}
  = 4(13^{2}-5^{2})
\\
\implies 
AB 
& = \frac{169-25}{16}
  = \frac{169-25}{16}
  = 9
\end{align*}

