This appears as 2007 AIME I Problems/Problem 8.

Let $a$ and $b$ satisfy $P(x)=Q_{1}(x)(2x+a)$ and $P(x)=Q_{2}(x)(x+b)$. We have
\begin{align*}
P(x) 
= (x^{2} + (k-29)x - k) (2x + a)
= (2x^{2} + (2k-43)x + k) (x + b)
\end{align*}

Equating coefficients:
\begin{align*}
\left\{\begin{aligned}
a + 2(k-29) 
& = 2b + (2k-43)
\\
a(k-29) - 2k
& = b(2k-43) + k
\\
-ak 
& = bk
\end{aligned}\right.
\end{align*}
\begin{align*}
\left\{\begin{aligned}
a - 2b
& = 15
\\
(a - 2b)k - 3k
& = 29a - 43b
\\
a
& = - b
\end{aligned}\right.
\implies
15k - 3k = 12k = 29a - 43b
= 72a
\implies 
k = 6a = 30
\end{align*}
\fbox{$k=30$.}
