Solve for $x\in\mathbb{R}$, where $3^{x}-2^{x}=65$.

\begin{answer}
\begin{flalign*}
3^{x} - 2^{x} 
& = 65
\\ 
(3^{x/2})^{2} - (2^{x/2})^{2}
& = 5 \times 13
\\
(3^{x/2} - 2^{x/2}) \times (3^{x/2} + 2^{x/2})
& = 5 \times 13
\end{flalign*}
Equating the factors on each side of the equality
\begin{flalign*}
\begin{cases}
3^{x/2} - 2^{x/2} & = 5
\\[1ex]
3^{x/2} + 2^{x/2} & = 13
\end{cases}
\implies 
2 \times 2^{x/2} & = 13 - 5 = 8
\implies
2^{x/2} = 2^{2}
\implies
x/2 = 2
\implies
x = 4
\end{flalign*}
\end{answer}
