If $x$ satisfies $x^{2}+\dfrac{1}{x^{2}}=\sqrt{2}$, evaluate $x^{2024}-\dfrac{1}{x^{2024}}$.

\begin{answer}

\begin{flalign*}
& x^{2}+\frac{1}{x^{2}}
= \sqrt{2}
\implies
\left(x^{2}+\frac{1}{x^{2}}\right)^{2}
= (\sqrt{2})^{2}
\implies
x^{4} + 2 x^{2}\frac{1}{x^{2}} + \frac{1}{x^{4}}
= 2
\implies
x^{4} + \frac{1}{x^{4}}
= 0
& \\
& \implies
x^{8} = -1
\implies
(x^{8})^{253} = (-1)^{253}
\implies
x^{2024} = -1
\implies
x^{2024} - \frac{1}{x^{2024}}
= -1 - \frac{1}{-1}
= 0
&
\end{flalign*}
\end{answer}
