\begin{align*}
a 
& = 99 \cdot 0.9 + 999 \cdot 0.9 + \ldots + 99{\ldots}9 \cdot 0.9
\\
& = 0.9 (99 + 999 + \ldots + 99{\ldots}9)
\\
& = 0.9 ((10^{2}-1) + (10^{3}-1) + \ldots + (10^{n}-1))
\\
& = (9/10) \cdot (10^{2}+10^{3}+\ldots+10^{n}-(n-1))
\\
& = 9 \cdot (10+10^{2}+\ldots+10^{n-1}-(n-1)/10)
\\
n = 101
\to 
a
& = 9 \cdot (10+10^{2}+\ldots+10^{100}-100/10)
\\
& = 9 \cdot (10^{2}+\ldots+10^{100})
\\
& = 900 \cdot (1+10+\ldots+10^{98})
\\
& = 900 \cdot \frac{1-10^{99}}{1-10}
\\
& = 100 \cdot (10^{99}-1)
\\
& = 10^{101}-100
\end{align*}