\begin{align*}
(z-r)^{3} & = z^{3} - 3rz^{2} + 3r^{2}z - r^{3}
\\
(z-\rho)^{3} & = z^{3} - 3\rho z^{2} + 3\rho^{2}z - \rho^{3}
\end{align*}

\begin{align*}
-3r 
& = M
\\
3r^{2} 
& = P
\\
-1 
& = G
\end{align*}
Likewise
\begin{align*}
-3\rho 
& = G
\\
3\rho^{2} 
& = P
\\
-1 
& = M
\end{align*}

The number of distinct triples $(M,P,G)$ is the number of triples $(-1,P,-1)$. 
\begin{align*}
M & = -1 \implies -3r = -1 \implies r = 1/3 \implies P = 1(1/3)^{2} = 1/3
\\
G & = -1 \implies -3\rho = -1 \implies \rho = 1/3 \implies P = 1(1/3)^{2} = 1/3
\end{align*}

Solution: $(-1,1/3,-1)$. 
